FiniteField broken

theories/algebra/Characteristic.ec
@@ -1,5 +1,6 @@
 require import AllCore Ring Int IntDiv.
 (*TODO: merge the hakyber proofs, argmin stuff needed.*)
+(*---*) import StdOrder.IntOrder IntID.
 
 
 abstract theory ComRing_Characteristic.
@@ -17,13 +18,13 @@ abstract theory ComRing_Characteristic.
   qed.
 
   lemma eq0_ofint_char : ofint char = zeror.
-  proof.
-    admit.
-  qed.
-
+  proof.      
+    admit.    
+  qed.	      
+	      
   (*TODO: should be in ZModule if all was good.*)
   lemma mulrM (x : t) (m n : int) : intmul x (m * n) = intmul (intmul x m) n.
-  proof.
+  proof.      
     wlog: m n / 0 <= n => [wlog|].
     + case (0 <= n); [by apply/wlog|].
       rewrite -ltzNge => gt0_n.
@@ -32,25 +33,29 @@ abstract theory ComRing_Characteristic.
       by rewrite mulrNN !mulrNz mulNrz opprK.
     elim: n => //= [|n le0n]; [by rewrite !mulr0z|].
     by rewrite mulrDr /= mulrSz mulrDz addrC => ->.
-  qed.
-
-  (*TODO: and this should be in ComRing. Also I have the feeling I already did that somewhere.*)
-  lemma mulr_int m n : ofint m * ofint n = ofint (m * n).
-  proof. by rewrite mulr_intr /ofint mulrM. qed.
-
+  qed.	      
+	      
   lemma dvd_char n : char %| n <=> ofint n = zeror.
-  proof.
-    split => [/dvdzP [q] ->>|].
-    + by rewrite -mulr_int eq0_ofint_char mulr0.
-    admit.
-  qed.
-
+  proof.      
+    split => [/dvdzP [q] ->>|]; [by rewrite -mulrz eq0_ofint_char mulr0|].
+    rewrite {1}(divz_eq n char) addrz -mulrz eq0_ofint_char mulr0 add0r.
+    move => eq_ofint.
+    admit.    
+  qed.	      
+	      
   lemma dvd2_char (m n : int) : char %| (m - n) <=> ofint m = ofint n.
   proof. by rewrite dvd_char /ofint mulrDz mulrNz subr_eq0. qed.
-
+	      
+  lemma char0P : char = 0 <=> injective ofint.
+  proof.      
+    split => [eq_char_0 x y /dvd2_char|inj_ofint].
+    + by rewrite eq_char_0 => /dvd0z /IntID.subr_eq0.
+    by move: (dvd2_char char 0); rewrite /= dvdzz /=; apply/inj_ofint.
+  qed.	      
+	      
 end ComRing_Characteristic.
-
-
+	      
+	      
 abstract theory IDomain_Characteristic.
 
   clone import IDomain as ID.
@@ -59,8 +64,74 @@ abstract theory IDomain_Characteristic.
 
   lemma char_integral : char = 0 \/ prime char.
   proof.
-    admit.
+    case/ler_eqVlt: ge0_char => [-> //|lt0char]; right.
+    move/ltzE/ler_eqVlt: lt0char; rewrite /= eq_sym neq1_char /=.
+    move => lt1char; split => // y /dvdzP [x] eq_char.
+    move: (congr1 ofint _ _ eq_char); rewrite -mulrz eq0_ofint_char eq_sym.
+    case/mulf_eq0 => /dvd_char /dvdzP [q ->>]; move/IntID.subr_eq0: eq_char.
+    + rewrite mulrAC -{1}(IntID.mul1r char) -mulNr -mulrDl.
+      case/IntID.mulf_eq0; [|by move => eq_; move: eq_ lt1char => ->].
+      by move/IntID.subr_eq0 => eq1; left; apply/dvdz1/dvdzP; exists q.
+    rewrite mulrA -{1}(IntID.mul1r char) -mulNr -mulrDl.
+    case/IntID.mulf_eq0; [|by move => eq_; move: eq_ lt1char => ->].
+    move/IntID.subr_eq0 => eq1; right; rewrite normrM (ger0_norm char) ?ge0_char //.
+    apply/IntID.subr_eq0; rewrite -{2}(IntID.mul1r char) -mulNr -mulrDl.
+    by apply/IntID.mulf_eq0; left; apply/IntID.subr_eq0/dvdz1/dvdzP; exists x.
   qed.
+
+  section Frobenius.
+
+    declare axiom prime_char : prime char.
+
+    op frobenius x = ID.exp x char.
+
+    lemma frobenius0 :
+      frobenius zeror = zeror.
+    proof. by rewrite /frobenius expr0z; move: prime_char => /gt0_prime /gtr_eqF ->. qed.
+
+    lemma frobenius1 :
+      frobenius oner = oner.
+    proof. by rewrite /frobenius expr1z. qed.
+
+    lemma frobenius_add (x y : t) :
+      frobenius (x + y) = frobenius x + frobenius y.
+    proof.
+      admit.
+    qed.
+
+    lemma frobenius_opp (x : t) :
+      frobenius (-x) = - frobenius x.
+    proof.
+      rewrite /frobenius -{1}(mul1r x) -mulNr exprMn ?ge0_char //.
+      rewrite -signr_odd ?ge0_char //.
+      admit.
+    qed.
+
+    lemma frobenius_mul (x y : t) :
+      frobenius (x * y) = frobenius x * frobenius y.
+    proof.
+      admit.
+    qed.
+
+    lemma frobenius_invr (x : t) :
+      frobenius (invr x) = invr (frobenius x).
+    proof.
+      admit.
+    qed.
+
+    lemma frobenius_unit (x : t) :
+      unit x <=> unit (frobenius x).
+    proof.
+      admit.
+    qed.
+
+    lemma bijective_frobenius :
+      bijective frobenius.
+    proof.
+      admit.
+    qed.
+  
+  end section Frobenius.
 
 end IDomain_Characteristic.
 
@@ -69,7 +140,6 @@ abstract theory Field_Characteristic.
 
   clone import Field as F.
 
-  (*TODO: I am bad at clones, check.*)
   clone include IDomain_Characteristic with
     theory ID <- F.
 
