theories/algebra/PolyFF.ec
@@ -15,6 +15,11 @@ end PolyFF.
 abstract theory FFQuotient.
 
   (*TODO: I should be able to find this, and then clone include it and link it to Polynomials and irreducible polynomials, and show that this is a field.*)
-  print RingQuotient.
+  clone import PolyFF as PFF.
+
+  print IdealComRing.
+  clone include IdealComRing with type t <- poly, theory IComRing <- PolyComRing.
+
+  print IdealComRing. print RingQuotient.
 
 end FFQuotient.
